Let's simplify the given grammar by removing useless symbols.

Given grammar:
1. \( S \rightarrow AB|CA \)
2. \( A \rightarrow a \)
3. \( B \rightarrow BC|AB \)
4. \( C \rightarrow ab|b \)

**Step 1:** Identify non-terminals from which terminals can be derived.

Starting with the given productions:
1. From \( A \), we can derive the terminal \( a \).
2. From \( C \), we can derive the terminals \( ab \) and \( b \).

Thus, initially, \( \{A, C\} \) are the non-terminals from which terminals can be derived.

Using the above information, we can further deduce:
1. From \( B \), using the production \( B \rightarrow BC \), we can derive \( b \) since \( C \) derives \( b \).
2. From \( S \), using the production \( S \rightarrow AB \), we can derive \( a \) and \( b \) since both \( A \) and \( B \) can derive terminals.

After this iteration, the set of non-terminals from which terminals can be derived becomes \( \{A, B, C\} \). No new non-terminals can be added, so we move to the next step.

**Step 2:** Identify non-terminals that are reachable from the start symbol.

Starting from \( S \):
1. \( S \) can reach \( A \) and \( B \) using the production \( S \rightarrow AB \).
2. \( S \) can also reach \( C \) using the production \( S \rightarrow CA \).
3. \( B \) can reach \( A \) and \( C \) using the production \( B \rightarrow AB \) and \( B \rightarrow BC \), respectively.

Therefore, all non-terminals \( \{A, B, C\} \) are reachable from \( S \).

**Step 3:** Eliminate useless symbols.

From the above steps, all non-terminals \( \{A, B, C\} \) are useful as they can derive terminals and are reachable from \( S \). So, we don't need to remove any production.

**Final Simplified Grammar:**
1. \( S \rightarrow AB|CA \)
2. \( A \rightarrow a \)
3. \( B \rightarrow BC|AB \)
4. \( C \rightarrow ab|b \)

The grammar remains unchanged as all the symbols are useful.

Alright! Let's work on the given grammar for question 2.

Given grammar:
1. \( S \rightarrow ASB|\varepsilon \)
2. \( A \rightarrow aAS|a \)
3. \( B \rightarrow SbS|A|bb \)

### a. Elimineer \( \varepsilon \)-productieregels.

To eliminate the \( \varepsilon \)-productions (productions that generate the empty string), we first identify the nullable variables (non-terminals that can produce \( \varepsilon \)).

From the given grammar, we can deduce:
1. \( S \) is nullable because \( S \rightarrow \varepsilon \).
2. \( B \) is nullable because \( B \rightarrow A \) and \( A \rightarrow a \), but \( A \) does not produce \( \varepsilon \), so we don't consider \( A \) as nullable.

Now, we will add new productions for the nullable variables:

1. \( S \rightarrow ASB|A|SB|SbS|B \)
2. \( A \rightarrow aAS|aA|aS|a \)
3. \( B \rightarrow SbS|Sb|bS|A|bb \)

### b. Elimineer unit producties.

To eliminate unit productions, we will first identify all unit pairs:

1. \( (S, A) \): From \( S \rightarrow A \)
2. \( (S, B) \): From \( S \rightarrow B \)
3. \( (B, A) \): From \( B \rightarrow A \)

Now, replace the unit productions with equivalent productions:

For \( S \rightarrow A \), we add:
1. \( S \rightarrow aAS|aA|aS|a \)

For \( S \rightarrow B \), we add:
1. \( S \rightarrow SbS|Sb|bS|bb \)

For \( B \rightarrow A \), we add:
1. \( B \rightarrow aAS|aA|aS|a \)

### c. Zijn er nutteloze symbolen? Zo ja elimineer ze.

By looking at the grammar, all symbols can produce terminal strings and are reachable from the start symbol. So, there are no useless symbols.

### d. Zet de grammatica om in CNF (Chomsky Normal Form).

To convert the grammar to CNF, we need to ensure that every production is of the form \( A \rightarrow BC \) or \( A \rightarrow a \), where A, B, and C are non-terminals and a is a terminal.

For simplicity, we'll introduce new non-terminals for terminals:
1. \( X_a \rightarrow a \)
2. \( X_b \rightarrow b \)

Now, replace terminals in the grammar:

1. \( S \rightarrow AX_aS|X_aA|AS|X_a \)
2. \( A \rightarrow X_aAX_a|X_aA|X_aS|X_a \)
3. \( B \rightarrow SS|SX_b|X_bS|X_bX_b \)

Now, further break down productions that aren't in CNF:

1. \( S \rightarrow AX_aS|X_aA|AS|X_a \)
2. \( A \rightarrow X_aAX_a|X_aA|X_aS|X_a \)
3. \( B \rightarrow SS|SX_b|X_bS|X_bX_b \)
4. \( S1 \rightarrow AX_a \) (New production)
5. \( A1 \rightarrow AX_a \) (New production)
6. \( B1 \rightarrow X_bS \) (New production)

Replace productions in the grammar:

1. \( S \rightarrow S1S|X_aA|AS|X_a \)
2. \( A \rightarrow A1X_a|X_aA|X_aS|X_a \)
3. \( B \rightarrow SS|SX_b|B1|X_bX_b \)
4. \( S1 \rightarrow AX_a \)
5. \( A1 \rightarrow AX_a \)
6. \( B1 \rightarrow X_bS \)

Now, the grammar is in CNF. 


